Kettenregel
Berechnen Sie zusammen die Ableitung der Funktion:
\,
k(x)=(x^2&-4x+1)^2&k'(x)=2(x^2-4x+1)\cdot (2x-4)
k(x)=(2x^3-x^2&+0,5x-3)^2&k'(x)=2(2x^3-x^2+0,5x-3)\cdot (6x^2-2x+0,5)
k(x)=(4x&-7)^2&k'(x)=2(4x-7)\cdot (4)
k(x)=(4x^2&+7x-1)^2&k'(x)=2(4x^2+7x-1)\cdot (8x+7)
k(x)=(x^2-4x&+4)^2&k'(x)=2(x^2-4x+4)\cdot (2x-4)
k(x)=(-x^2&+4)^2&k'(x)=2(-x^2+4)\cdot (-2x)
k(x)=(6x&+3)^2&k'(x)=2(6x+3)\cdot (6)
k(x)=(\sqrt{x}&-2)^2&k'(x)=2(\sqrt{x}-2)\cdot (0,5x^{-1/2})
k(x)=(x^2&+2\sqrt{x})^2&k'(x)=2(x^2+2\sqrt{x})\cdot (2x+x^{-1/2})
k(x)=(x^2&-4x+1)^3&k'(x)=3(x^2-4x+1)^2\cdot (2x-4)
k(x)=(2x^3-x^2&+0,5x-3)^3&k'(x)=3(2x^3-x^2+0,5x-3)^2\cdot (6x^2-2x+0,5)
k(x)=(4x&-7)^3&k'(x)=3(4x-7)^2\cdot (4)
k(x)=(4x^2&+7x-1)^3&k'(x)=3(4x^2+7x-1)^2\cdot (8x+7)
k(x)=(x^2-4x&+4)^3&k'(x)=3(x^2-4x+4)^2\cdot (2x-4)
k(x)=(-x^2&+4)^3&k'(x)=3(-x^2+4)^2\cdot (-2x)
k(x)=(6x&+3)^3&k'(x)=3(6x+3)^2\cdot (6)
k(x)=(\sqrt{x}&-2)^3&k'(x)=3(\sqrt{x}-2)^2\cdot (0,5x^{-1/2})
k(x)=(x^2&+2\sqrt{x})^3&k'(x)=3(x^2+2\sqrt{x})^2\cdot (2x+x^{-1/2})
k(x)=1/(x^2&-4x+1)&k'(x)=-(x^2-4x+1)^{-2}\cdot (2x-4)
k(x)=1/(2x^3-x^2&+0,5x-3)&k'(x)=-(2x^3-x^2+0,5x-3)^{-2}\cdot (6x^2-2x+0,5)
k(x)=1/(4x&-7)&k'(x)=-(4x-7)^{-2}\cdot (4)
k(x)=1/(4x^2&+7x-1)&k'(x)=-(4x^2+7x-1)^{-2}\cdot (8x+7)
k(x)=1/(x^2-4x&+4)&k'(x)=-(x^2-4x+4)^{-2}\cdot (2x-4)
k(x)=1/(-x^2&+4)&k'(x)=-(-x^2+4)^{-2}\cdot (-2x)
k(x)=1/(6x&+3)&k'(x)=-(6x+3)^{-2}\cdot (6)
k(x)=1/(\sqrt{x}&-2)&k'(x)=-(\sqrt{x}-2)^{-2}\cdot (0,5x^{-1/2})
k(x)=1/(x^2&+2\sqrt{x})&k'(x)=-(x^2+2\sqrt{x})^{-2}\cdot (2x+x^{-1/2})
k(x)=(x^2&-4x+1)^5&k'(x)=5(x^2-4x+1)^4\cdot (2x-4)
k(x)=(2x^3-x^2&+0,5x-3)^5&k'(x)=5(2x^3-x^2+0,5x-3)^4\cdot (6x^2-2x+0,5)
k(x)=(4x&-7)^5&k'(x)=5(4x-7)^4\cdot (4)
k(x)=(4x^2&+7x-1)^5&k'(x)=5(4x^2+7x-1)^4\cdot (8x+7)
k(x)=(x^2-4x&+4)^5&k'(x)=5(x^2-4x+4)^4\cdot (2x-4)
k(x)=(-x^2&+4)^5&k'(x)=5(-x^2+4)^4\cdot (-2x)
k(x)=(6x&+3)^5&k'(x)=5(6x+3)^4\cdot (6)
k(x)=(\sqrt{x}&-2)^5&k'(x)=5(\sqrt{x}-2)^4\cdot (0,5x^{-1/2})
k(x)=(x^2&+2\sqrt{x})^5&k'(x)=5(x^2+2\sqrt{x})^4\cdot (2x+x^{-1/2})
k(x)=(x^2&-4x+1)^{1/2}&k'(x)=0,5(x^2-4x+1)^{-1/2}\cdot (2x-4)
k(x)=(2x^3-x^2&+0,5x-3)^{1/2}&k'(x)=0,5(2x^3-x^2+0,5x-3)^{-1/2}\cdot (6x^2-2x+0,5)
k(x)=(4x&-7)^{1/2}&k'(x)=0,5(4x-7)^{-1/2}\cdot (4)
k(x)=(4x^2&+7x-1)^{1/2}&k'(x)=0,5(4x^2+7x-1)^{-1/2}\cdot (8x+7)
k(x)=(x^2-4x&+4)^{1/2}&k'(x)=0,5(x^2-4x+4)^{-1/2}\cdot (2x-4)
k(x)=(-x^2&+4)^{1/2}&k'(x)=0,5(-x^2+4)^{-1/2}\cdot (-2x)
k(x)=(6x&+3)^{1/2}&k'(x)=0,5(6x+3)^{-1/2}\cdot (6)
k(x)=(\sqrt{x}&-2)^{1/2}&k'(x)=0,5(\sqrt{x}-2)^{-1/2}\cdot (0,5x^{-1/2})
k(x)=(x^2&+2\sqrt{x})^{1/2}&k'(x)=0,5(x^2+2\sqrt{x})^{-1/2}\cdot (2x+x^{-1/2})