Produktregel
Berechnen Sie zusammen die Ableitung der Funktion und vereinfachen Sie den Term
\cdot\mbox{}
f(x)=x&e^x&f’(x)=(x+1)e^x
f(x)=e^x&e^x&f’(x)=2e^x\cdot e^x
f(x)=(2x+1)&e^x&f’(x)=(2x+3)e^x
f(x)=\sqrt{x}&e^x&f’(x)=(x^{1/2}+0,5x^{-1/2})e^x
f(x)=(e^x-2)&(2+x^2)&f’(x)=(x^2+2x+2)e^x-4x
f(x)=e^x&(1+e^x)&f’(x)=(1+2e^x)e^x
f(x)=0,5x^2&e^x&f’(x)=(0,5x^2+x)e^x
f(x)=4x&e^x&f’(x)=4(x+1)e^x
f(x)=\frac{1}{x}&e^x&f’(x)=\left(\frac{1}{x}-\frac{1}{x^2}\right)e^x
f(x)=\frac{1}{3}x^3&e^x&f’(x)=\left(\frac{1}{3}x^3+x^2\right)e^x
f(x)=e^x&(e^x-2)&f’(x)=2e^x(e^x-1)
f(x)=(x^2-2x+1)&e^x&f’(x)=(x^2-1)e^x
f(x)=(e^x+1)&(e^x-1)&f’(x)=2e^x\cdot e^x
f(x)=x^4&e^x&f’(x)=(x^4+4x^3)e^x
f(x)=2e^x&(e^x-1)&f’(x)=2e^x(2e^x-1)