Quadratische Erg√§nzung
$f(x)$ ist die Summe der beiden quadratischen Funktionen $f(x)=f_1(x)+f_2(x)$. Bestimmt \emph{zusammen} $f(x)$ in Scheitelpunktform und den Scheitelpunkt $(d|e)$ von $f(x)$.
\mbox{ }und\mbox{ }
$f_1(x)=\frac{1}{2}x^2+1x+20$&$f_2(x)=\frac{1}{2}x^2+11x+10$&$S(-6|-6)$
$f_1(x)=\frac{1}{2}x^2+4x+20$&$f_2(x)=\frac{1}{2}x^2+8x+11$&$S(-6|-5)$
$f_1(x)=\frac{1}{2}x^2+4x+11$&$f_2(x)=\frac{1}{2}x^2+8x+21$&$S(-6|-4)$
$f_1(x)=\frac{1}{2}x^2+7x+15$&$f_2(x)=\frac{1}{2}x^2+5x+18$&$S(-6|-3)$
$f_1(x)=\frac{1}{2}x^2+7x+15$&$f_2(x)=\frac{1}{2}x^2+5x+19$&$S(-6|-2)$
$f_1(x)=\frac{1}{2}x^2+1x+14$&$f_2(x)=\frac{1}{2}x^2+11x+21$&$S(-6|-1)$
$f_1(x)=\frac{1}{2}x^2+4x+15$&$f_2(x)=\frac{1}{2}x^2+8x+22$&$S(-6|1)$
$f_1(x)=\frac{1}{2}x^2+10x+14$&$f_2(x)=\frac{1}{2}x^2+2x+24$&$S(-6|2)$
$f_1(x)=\frac{1}{2}x^2+7x+22$&$f_2(x)=\frac{1}{2}x^2+5x+17$&$S(-6|3)$
$f_1(x)=\frac{1}{2}x^2+8x+25$&$f_2(x)=\frac{1}{2}x^2+4x+15$&$S(-6|4)$
$f_1(x)=\frac{1}{2}x^2+5x+26$&$f_2(x)=\frac{1}{2}x^2+7x+15$&$S(-6|5)$
$f_1(x)=\frac{1}{2}x^2+7x+19$&$f_2(x)=\frac{1}{2}x^2+5x+23$&$S(-6|6)$
$f_1(x)=\frac{1}{2}x^2+6x+5$&$f_2(x)=\frac{1}{2}x^2+4x+14$&$S(-5|-6)$
$f_1(x)=\frac{1}{2}x^2+5x+5$&$f_2(x)=\frac{1}{2}x^2+5x+15$&$S(-5|-5)$
$f_1(x)=\frac{1}{2}x^2+7x+7$&$f_2(x)=\frac{1}{2}x^2+3x+14$&$S(-5|-4)$
$f_1(x)=\frac{1}{2}x^2+8x+7$&$f_2(x)=\frac{1}{2}x^2+2x+15$&$S(-5|-3)$
$f_1(x)=\frac{1}{2}x^2+1x+16$&$f_2(x)=\frac{1}{2}x^2+9x+7$&$S(-5|-2)$
$f_1(x)=\frac{1}{2}x^2+5x+17$&$f_2(x)=\frac{1}{2}x^2+5x+7$&$S(-5|-1)$
$f_1(x)=\frac{1}{2}x^2+4x+18$&$f_2(x)=\frac{1}{2}x^2+6x+8$&$S(-5|1)$
$f_1(x)=\frac{1}{2}x^2+3x+13$&$f_2(x)=\frac{1}{2}x^2+7x+14$&$S(-5|2)$
$f_1(x)=\frac{1}{2}x^2+6x+9$&$f_2(x)=\frac{1}{2}x^2+4x+19$&$S(-5|3)$
$f_1(x)=\frac{1}{2}x^2+5x+11$&$f_2(x)=\frac{1}{2}x^2+5x+18$&$S(-5|4)$
$f_1(x)=\frac{1}{2}x^2+1x+12$&$f_2(x)=\frac{1}{2}x^2+9x+18$&$S(-5|5)$
$f_1(x)=\frac{1}{2}x^2+6x+16$&$f_2(x)=\frac{1}{2}x^2+4x+15$&$S(-5|6)$
$f_1(x)=\frac{1}{2}x^2+4x+5$&$f_2(x)=\frac{1}{2}x^2+4x+5$&$S(-4|-6)$
$f_1(x)=\frac{1}{2}x^2+4x+8$&$f_2(x)=\frac{1}{2}x^2+4x+3$&$S(-4|-5)$
$f_1(x)=\frac{1}{2}x^2+1x+5$&$f_2(x)=\frac{1}{2}x^2+7x+7$&$S(-4|-4)$
$f_1(x)=\frac{1}{2}x^2+2x+4$&$f_2(x)=\frac{1}{2}x^2+6x+9$&$S(-4|-3)$
$f_1(x)=\frac{1}{2}x^2+4x+4$&$f_2(x)=\frac{1}{2}x^2+4x+10$&$S(-4|-2)$
$f_1(x)=\frac{1}{2}x^2-1x+11$&$f_2(x)=\frac{1}{2}x^2+9x+4$&$S(-4|-1)$
$f_1(x)=\frac{1}{2}x^2-1x+7$&$f_2(x)=\frac{1}{2}x^2+9x+10$&$S(-4|1)$
$f_1(x)=\frac{1}{2}x^2+3x+12$&$f_2(x)=\frac{1}{2}x^2+5x+6$&$S(-4|2)$
$f_1(x)=\frac{1}{2}x^2+3x+6$&$f_2(x)=\frac{1}{2}x^2+5x+13$&$S(-4|3)$
$f_1(x)=\frac{1}{2}x^2+1x+7$&$f_2(x)=\frac{1}{2}x^2+7x+13$&$S(-4|4)$
$f_1(x)=\frac{1}{2}x^2+7x+14$&$f_2(x)=\frac{1}{2}x^2+1x+7$&$S(-4|5)$
$f_1(x)=\frac{1}{2}x^2+5x+7$&$f_2(x)=\frac{1}{2}x^2+3x+15$&$S(-4|6)$
$f_1(x)=\frac{1}{2}x^2+7x-3$&$f_2(x)=\frac{1}{2}x^2-1x+6$&$S(-3|-6)$
$f_1(x)=\frac{1}{2}x^2+1x+7$&$f_2(x)=\frac{1}{2}x^2+5x-3$&$S(-3|-5)$
$f_1(x)=\frac{1}{2}x^2+7x+6$&$f_2(x)=\frac{1}{2}x^2-1x-1$&$S(-3|-4)$
$f_1(x)=\frac{1}{2}x^2+3x+3$&$f_2(x)=\frac{1}{2}x^2+3x+3$&$S(-3|-3)$
$f_1(x)=\frac{1}{2}x^2+5x-1$&$f_2(x)=\frac{1}{2}x^2+1x+8$&$S(-3|-2)$
$f_1(x)=\frac{1}{2}x^2+7x+5$&$f_2(x)=\frac{1}{2}x^2-1x+3$&$S(-3|-1)$
$f_1(x)=\frac{1}{2}x^2-1x+9$&$f_2(x)=\frac{1}{2}x^2+7x+1$&$S(-3|1)$
$f_1(x)=\frac{1}{2}x^2+5x+3$&$f_2(x)=\frac{1}{2}x^2+1x+8$&$S(-3|2)$
$f_1(x)=\frac{1}{2}x^2+5x+11$&$f_2(x)=\frac{1}{2}x^2+1x+1$&$S(-3|3)$
$f_1(x)=\frac{1}{2}x^2+2x+9$&$f_2(x)=\frac{1}{2}x^2+4x+4$&$S(-3|4)$
$f_1(x)=\frac{1}{2}x^2+1x+5$&$f_2(x)=\frac{1}{2}x^2+5x+9$&$S(-3|5)$
$f_1(x)=\frac{1}{2}x^2+2x+6$&$f_2(x)=\frac{1}{2}x^2+4x+9$&$S(-3|6)$
$f_1(x)=\frac{1}{2}x^2+5x+4$&$f_2(x)=\frac{1}{2}x^2-1x-6$&$S(-2|-6)$
$f_1(x)=\frac{1}{2}x^2+3x+4$&$f_2(x)=\frac{1}{2}x^2+1x-5$&$S(-2|-5)$
$f_1(x)=\frac{1}{2}x^2-1x-3$&$f_2(x)=\frac{1}{2}x^2+5x+3$&$S(-2|-4)$
$f_1(x)=\frac{1}{2}x^2-1x+6$&$f_2(x)=\frac{1}{2}x^2+5x-5$&$S(-2|-3)$
$f_1(x)=\frac{1}{2}x^2+7x-2$&$f_2(x)=\frac{1}{2}x^2-3x+4$&$S(-2|-2)$
$f_1(x)=\frac{1}{2}x^2+3x-2$&$f_2(x)=\frac{1}{2}x^2+1x+5$&$S(-2|-1)$
$f_1(x)=\frac{1}{2}x^2+5x+1$&$f_2(x)=\frac{1}{2}x^2-1x+4$&$S(-2|1)$
$f_1(x)=\frac{1}{2}x^2+7x+4$&$f_2(x)=\frac{1}{2}x^2-3x+2$&$S(-2|2)$
$f_1(x)=\frac{1}{2}x^2-3x+3$&$f_2(x)=\frac{1}{2}x^2+7x+4$&$S(-2|3)$
$f_1(x)=\frac{1}{2}x^2+1x+3$&$f_2(x)=\frac{1}{2}x^2+3x+5$&$S(-2|4)$
$f_1(x)=\frac{1}{2}x^2-2x+5$&$f_2(x)=\frac{1}{2}x^2+6x+4$&$S(-2|5)$
$f_1(x)=\frac{1}{2}x^2+2x+8$&$f_2(x)=\frac{1}{2}x^2+2x+2$&$S(-2|6)$
$f_1(x)=\frac{1}{2}x^2+3x-1$&$f_2(x)=\frac{1}{2}x^2-1x-4$&$S(-1|-6)$
$f_1(x)=\frac{1}{2}x^2+6x-7$&$f_2(x)=\frac{1}{2}x^2-4x+3$&$S(-1|-5)$
$f_1(x)=\frac{1}{2}x^2+6x-4$&$f_2(x)=\frac{1}{2}x^2-4x+1$&$S(-1|-4)$
$f_1(x)=\frac{1}{2}x^2+5x+1$&$f_2(x)=\frac{1}{2}x^2-3x-3$&$S(-1|-3)$
$f_1(x)=\frac{1}{2}x^2-3x+4$&$f_2(x)=\frac{1}{2}x^2+5x-5$&$S(-1|-2)$
$f_1(x)=\frac{1}{2}x^2-1x+1$&$f_2(x)=\frac{1}{2}x^2+3x-1$&$S(-1|-1)$
$f_1(x)=\frac{1}{2}x^2+1x-4$&$f_2(x)=\frac{1}{2}x^2+1x+6$&$S(-1|1)$
$f_1(x)=\frac{1}{2}x^2+1x-3$&$f_2(x)=\frac{1}{2}x^2+1x+6$&$S(-1|2)$
$f_1(x)=\frac{1}{2}x^2-2x-1$&$f_2(x)=\frac{1}{2}x^2+4x+5$&$S(-1|3)$
$f_1(x)=\frac{1}{2}x^2-2x-2$&$f_2(x)=\frac{1}{2}x^2+4x+7$&$S(-1|4)$
$f_1(x)=\frac{1}{2}x^2+3x+5$&$f_2(x)=\frac{1}{2}x^2-1x+1$&$S(-1|5)$
$f_1(x)=\frac{1}{2}x^2+4x+1$&$f_2(x)=\frac{1}{2}x^2-2x+6$&$S(-1|6)$
$f_1(x)=\frac{1}{2}x^2+1x-6$&$f_2(x)=\frac{1}{2}x^2-3x+1$&$S(1|-6)$
$f_1(x)=\frac{1}{2}x^2-5x-6$&$f_2(x)=\frac{1}{2}x^2+3x+2$&$S(1|-5)$
$f_1(x)=\frac{1}{2}x^2+4x+2$&$f_2(x)=\frac{1}{2}x^2-6x-5$&$S(1|-4)$
$f_1(x)=\frac{1}{2}x^2+4x-6$&$f_2(x)=\frac{1}{2}x^2-6x+4$&$S(1|-3)$
$f_1(x)=\frac{1}{2}x^2+3x-2$&$f_2(x)=\frac{1}{2}x^2-5x+1$&$S(1|-2)$
$f_1(x)=\frac{1}{2}x^2+3x-4$&$f_2(x)=\frac{1}{2}x^2-5x+4$&$S(1|-1)$
$f_1(x)=\frac{1}{2}x^2+2x-1$&$f_2(x)=\frac{1}{2}x^2-4x+3$&$S(1|1)$
$f_1(x)=\frac{1}{2}x^2-3x-3$&$f_2(x)=\frac{1}{2}x^2+1x+6$&$S(1|2)$
$f_1(x)=\frac{1}{2}x^2+4x-1$&$f_2(x)=\frac{1}{2}x^2-6x+5$&$S(1|3)$
$f_1(x)=\frac{1}{2}x^2-3x-2$&$f_2(x)=\frac{1}{2}x^2+1x+7$&$S(1|4)$
$f_1(x)=\frac{1}{2}x^2-4x-2$&$f_2(x)=\frac{1}{2}x^2+2x+8$&$S(1|5)$
$f_1(x)=\frac{1}{2}x^2-3x+9$&$f_2(x)=\frac{1}{2}x^2+1x-2$&$S(1|6)$
$f_1(x)=\frac{1}{2}x^2-3x+2$&$f_2(x)=\frac{1}{2}x^2-1x-4$&$S(2|-6)$
$f_1(x)=\frac{1}{2}x^2-6x+3$&$f_2(x)=\frac{1}{2}x^2+2x-4$&$S(2|-5)$
$f_1(x)=\frac{1}{2}x^2+2x-5$&$f_2(x)=\frac{1}{2}x^2-6x+5$&$S(2|-4)$
$f_1(x)=\frac{1}{2}x^2-7x+5$&$f_2(x)=\frac{1}{2}x^2+3x-4$&$S(2|-3)$
$f_1(x)=\frac{1}{2}x^2+1x+3$&$f_2(x)=\frac{1}{2}x^2-5x-1$&$S(2|-2)$
$f_1(x)=\frac{1}{2}x^2-6x-2$&$f_2(x)=\frac{1}{2}x^2+2x+5$&$S(2|-1)$
$f_1(x)=\frac{1}{2}x^2-7x+8$&$f_2(x)=\frac{1}{2}x^2+3x-3$&$S(2|1)$
$f_1(x)=\frac{1}{2}x^2+2x+8$&$f_2(x)=\frac{1}{2}x^2-6x-2$&$S(2|2)$
$f_1(x)=\frac{1}{2}x^2-1x+5$&$f_2(x)=\frac{1}{2}x^2-3x+2$&$S(2|3)$
$f_1(x)=\frac{1}{2}x^2-2x+5$&$f_2(x)=\frac{1}{2}x^2-2x+3$&$S(2|4)$
$f_1(x)=\frac{1}{2}x^2-2x+10$&$f_2(x)=\frac{1}{2}x^2-2x-1$&$S(2|5)$
$f_1(x)=\frac{1}{2}x^2+1x+8$&$f_2(x)=\frac{1}{2}x^2-5x+2$&$S(2|6)$
$f_1(x)=\frac{1}{2}x^2-8x+6$&$f_2(x)=\frac{1}{2}x^2+2x-3$&$S(3|-6)$
$f_1(x)=\frac{1}{2}x^2-2x+5$&$f_2(x)=\frac{1}{2}x^2-4x-1$&$S(3|-5)$
$f_1(x)=\frac{1}{2}x^2-7x+8$&$f_2(x)=\frac{1}{2}x^2+1x-3$&$S(3|-4)$
$f_1(x)=\frac{1}{2}x^2-1x+7$&$f_2(x)=\frac{1}{2}x^2-5x-1$&$S(3|-3)$
$f_1(x)=\frac{1}{2}x^2-4x+4$&$f_2(x)=\frac{1}{2}x^2-2x+3$&$S(3|-2)$
$f_1(x)=\frac{1}{2}x^2-4x-1$&$f_2(x)=\frac{1}{2}x^2-2x+9$&$S(3|-1)$
$f_1(x)=\frac{1}{2}x^2-4x+7$&$f_2(x)=\frac{1}{2}x^2-2x+3$&$S(3|1)$
$f_1(x)=\frac{1}{2}x^2-3x+2$&$f_2(x)=\frac{1}{2}x^2-3x+9$&$S(3|2)$
$f_1(x)=\frac{1}{2}x^2+1x+2$&$f_2(x)=\frac{1}{2}x^2-7x+10$&$S(3|3)$
$f_1(x)=\frac{1}{2}x^2-4x+8$&$f_2(x)=\frac{1}{2}x^2-2x+5$&$S(3|4)$
$f_1(x)=\frac{1}{2}x^2-3x+10$&$f_2(x)=\frac{1}{2}x^2-3x+4$&$S(3|5)$
$f_1(x)=\frac{1}{2}x^2-7x+13$&$f_2(x)=\frac{1}{2}x^2+1x+2$&$S(3|6)$
$f_1(x)=\frac{1}{2}x^2-2x+3$&$f_2(x)=\frac{1}{2}x^2-6x+7$&$S(4|-6)$
$f_1(x)=\frac{1}{2}x^2-3x+3$&$f_2(x)=\frac{1}{2}x^2-5x+8$&$S(4|-5)$
$f_1(x)=\frac{1}{2}x^2-6x+6$&$f_2(x)=\frac{1}{2}x^2-2x+6$&$S(4|-4)$
$f_1(x)=\frac{1}{2}x^2-1x+6$&$f_2(x)=\frac{1}{2}x^2-7x+7$&$S(4|-3)$
$f_1(x)=\frac{1}{2}x^2-2x+11$&$f_2(x)=\frac{1}{2}x^2-6x+3$&$S(4|-2)$
$f_1(x)=\frac{1}{2}x^2-6x+9$&$f_2(x)=\frac{1}{2}x^2-2x+6$&$S(4|-1)$
$f_1(x)=\frac{1}{2}x^2-3x+9$&$f_2(x)=\frac{1}{2}x^2-5x+8$&$S(4|1)$
$f_1(x)=\frac{1}{2}x^2-5x+9$&$f_2(x)=\frac{1}{2}x^2-3x+9$&$S(4|2)$
$f_1(x)=\frac{1}{2}x^2+1x+11$&$f_2(x)=\frac{1}{2}x^2-9x+8$&$S(4|3)$
$f_1(x)=\frac{1}{2}x^2-9x+5$&$f_2(x)=\frac{1}{2}x^2+1x+15$&$S(4|4)$
$f_1(x)=\frac{1}{2}x^2-5x+14$&$f_2(x)=\frac{1}{2}x^2-3x+7$&$S(4|5)$
$f_1(x)=\frac{1}{2}x^2-4x+10$&$f_2(x)=\frac{1}{2}x^2-4x+12$&$S(4|6)$
$f_1(x)=\frac{1}{2}x^2-7x+14$&$f_2(x)=\frac{1}{2}x^2-3x+5$&$S(5|-6)$
$f_1(x)=\frac{1}{2}x^2-7x+5$&$f_2(x)=\frac{1}{2}x^2-3x+15$&$S(5|-5)$
$f_1(x)=\frac{1}{2}x^2-6x+6$&$f_2(x)=\frac{1}{2}x^2-4x+15$&$S(5|-4)$
$f_1(x)=\frac{1}{2}x^2-1x+16$&$f_2(x)=\frac{1}{2}x^2-9x+6$&$S(5|-3)$
$f_1(x)=\frac{1}{2}x^2-2x+8$&$f_2(x)=\frac{1}{2}x^2-8x+15$&$S(5|-2)$
$f_1(x)=\frac{1}{2}x^2-7x+9$&$f_2(x)=\frac{1}{2}x^2-3x+15$&$S(5|-1)$
$f_1(x)=\frac{1}{2}x^2-4x+16$&$f_2(x)=\frac{1}{2}x^2-6x+10$&$S(5|1)$
$f_1(x)=\frac{1}{2}x^2-5x+14$&$f_2(x)=\frac{1}{2}x^2-5x+13$&$S(5|2)$
$f_1(x)=\frac{1}{2}x^2-5x+16$&$f_2(x)=\frac{1}{2}x^2-5x+12$&$S(5|3)$
$f_1(x)=\frac{1}{2}x^2-6x+16$&$f_2(x)=\frac{1}{2}x^2-4x+13$&$S(5|4)$
$f_1(x)=\frac{1}{2}x^2-5x+14$&$f_2(x)=\frac{1}{2}x^2-5x+16$&$S(5|5)$
$f_1(x)=\frac{1}{2}x^2-2x+11$&$f_2(x)=\frac{1}{2}x^2-8x+20$&$S(5|6)$
$f_1(x)=\frac{1}{2}x^2-1x+19$&$f_2(x)=\frac{1}{2}x^2-11x+11$&$S(6|-6)$
$f_1(x)=\frac{1}{2}x^2-1x+14$&$f_2(x)=\frac{1}{2}x^2-11x+17$&$S(6|-5)$
$f_1(x)=\frac{1}{2}x^2-7x+13$&$f_2(x)=\frac{1}{2}x^2-5x+19$&$S(6|-4)$
$f_1(x)=\frac{1}{2}x^2-7x+15$&$f_2(x)=\frac{1}{2}x^2-5x+18$&$S(6|-3)$
$f_1(x)=\frac{1}{2}x^2-5x+12$&$f_2(x)=\frac{1}{2}x^2-7x+22$&$S(6|-2)$
$f_1(x)=\frac{1}{2}x^2-4x+22$&$f_2(x)=\frac{1}{2}x^2-8x+13$&$S(6|-1)$
$f_1(x)=\frac{1}{2}x^2-7x+19$&$f_2(x)=\frac{1}{2}x^2-5x+18$&$S(6|1)$
$f_1(x)=\frac{1}{2}x^2-8x+19$&$f_2(x)=\frac{1}{2}x^2-4x+19$&$S(6|2)$
$f_1(x)=\frac{1}{2}x^2-4x+16$&$f_2(x)=\frac{1}{2}x^2-8x+23$&$S(6|3)$
$f_1(x)=\frac{1}{2}x^2-10x+16$&$f_2(x)=\frac{1}{2}x^2-2x+24$&$S(6|4)$
$f_1(x)=\frac{1}{2}x^2-1x+22$&$f_2(x)=\frac{1}{2}x^2-11x+19$&$S(6|5)$
$f_1(x)=\frac{1}{2}x^2-5x+17$&$f_2(x)=\frac{1}{2}x^2-7x+25$&$S(6|6)$
